

# STAT 6530

## Homework 2

Spencer King  
811336941

Due: Monday, February 16 via eLC by 11:59 pm

### Problems

1. Consider the following study done at the National Institute of Science and Technology. Asbestos fibers on filters were counted as part of a project to develop measurement standards for asbestos concentration. Asbestos dissolved in water was spread on a filter, and 3-mm diameter punches were taken from the filter and mounted on a transmission electron microscope. An operator counted the number of fibers in each of 23 grid squares, yielding the following counts:

31 29 19 18 31 28 34 27 34 30 16 18  
26 27 27 18 24 22 28 24 21 17 24

We decide to model the counts as arising from a  $\text{Poisson}(\mu)$  distribution. The probability mass function for this distribution is:

$$f(y; \mu) = \frac{\mu^y e^{-\mu}}{y!}$$

for  $y = 0, 1, 2, \dots$ , and the distribution has mean and variance both equal to  $\mu$ , where the rate parameter  $\mu$  must be a positive real number.

- (a) (5 points) Find the maximum likelihood estimate of  $\mu$ . Show your work (don't just write the answer, even though we did this in class).

The likelihood function is

$$L(\mu) = \prod_{i=1}^n f(y_i; \mu) = \prod_{i=1}^n \frac{\mu^{y_i} e^{-\mu}}{y_i!}.$$

The log-likelihood function is

$$\ell(\mu) = \sum_{i=1}^n y_i \log(\mu) - n\mu - \sum_{i=1}^n \log(y_i!).$$

To find the maximum likelihood estimate, we take the derivative of the log-likelihood function with respect to  $\mu$  and set it equal to zero:

$$\frac{d\ell}{d\mu} = \sum_{i=1}^n \frac{y_i}{\mu} - n = 0$$

Solving for  $\mu$ , we get

$$\hat{\mu} = \frac{1}{n} \sum_{i=1}^n y_i = \frac{573}{23} \approx 24.913,$$

which is the sample mean of the counts. In this case, since the log-likelihood is concave in  $\mu$  for  $\mu > 0$ , the critical point found by setting the first derivative to zero is the unique global maximum, so a second derivative check is unnecessary.

(b) (5 points) Find an approximate 90% confidence interval for  $\mu$ .

In this case since an approximate confidence interval (CI) will do, we can use the Wald CI. Let's assume  $Y_1, \dots, Y_n \stackrel{iid}{\sim} \text{Poisson}(\mu)$ . Then

$$\mathbb{E}[Y_i] = \mu, \quad \text{Var}(Y_i) = \mu.$$

The sample mean is  $\bar{Y} = \frac{1}{n} \sum_{i=1}^n Y_i$ . By independence,

$$\text{Var}(\bar{Y}) = \frac{1}{n^2} \sum_{i=1}^n \text{Var}(Y_i) = \frac{1}{n^2} \cdot n\mu = \frac{\mu}{n}.$$

By the Central Limit Theorem,

$$\bar{Y} \approx N\left(\mu, \frac{\mu}{n}\right),$$

so

$$\frac{\bar{Y} - \mu}{\sqrt{\mu/n}} \approx N(0, 1).$$

Replacing  $\mu$  in the standard error by  $\bar{Y}$  gives the approximate CI

$$\mu \in \bar{Y} \pm z_{0.95} \sqrt{\frac{\bar{Y}}{n}}.$$

Here  $n = 23$  and  $\bar{Y} = \hat{\mu} = \frac{573}{23} \approx 24.913$ . So

$$\sqrt{\frac{\bar{Y}}{n}} = \sqrt{\frac{24.913}{23}} \approx 1.041.$$

Using  $z_{0.95} \approx 1.645$  for a 90% two-sided CI, the margin is

$$1.645(1.041) \approx 1.712,$$

hence the approximate 90% CI is

$$24.913 \pm 1.712 = (23.201, 26.625).$$

2. Consider an i.i.d. sample of size  $n$  from a distribution with probability mass function

$$f(y; p) = p(1 - p)^{y-1}$$

for  $y = 1, 2, 3, \dots$ , with  $0 < p \leq 1$ .

(a) (5 points) Find the maximum likelihood estimate of  $p$ .

The likelihood function is

$$L(p) = \prod_{i=1}^n f(y_i; p) = \prod_{i=1}^n p(1 - p)^{y_i-1} = p^n (1 - p)^{\sum_{i=1}^n y_i - n}$$

If we let  $\sum_{i=1}^n y_i - n = S - n$ , then the log-likelihood function is

$$\ell(p) = n \log(p) + (S - n) \log(1 - p)$$

Next, we need to take the first and second derivatives

$$\ell'(p) = \frac{n}{p} + \frac{S - n}{1 - p}$$

$$\ell''(p) = -\frac{n}{p^2} - \frac{S - n}{(1 - p)^2}$$

Now, we know that for  $\ell''(p) < 0$  for  $(0 < p < 1)$ . So,  $\ell$  is strictly concave on  $(0, 1)$ . Therefore, an interior solution to  $\ell'(p) = 0$  is the unique global maximizer on  $(0, 1)$ .

$$\ell'(p) = \frac{n}{p} + \frac{S - n}{1 - p} = 0$$

$$p(S - n) = n(1 - p)$$

$$pS - pn = n - np$$

$$\hat{p} = \frac{n}{S}$$

We must now check the boundary  $p = 1$ . If  $S > n$  (i.e., at least one  $y_i > 1$ ), then  $S - n > 0$  and

$$L(1) = 1^n \cdot 0^{S-n} = 0$$

so the maximizer must be interior and  $\hat{p} = \frac{n}{S} \in (0, 1)$ . If  $S = n$  (i.e., all  $y_i = 1$ ), the  $L(p) = p^n$ , which is increasing on  $(0, 1]$ , so the maximum occurs at  $p = 1$ . Thus the final MLE is as follows:

$$\hat{p} = \begin{cases} \frac{n}{\sum_{i=1}^n y_i}, & \text{if } \sum_{i=1}^n y_i > n, \\ 1, & \text{if } \sum_{i=1}^n y_i = n. \end{cases} = \min\left(1, \frac{n}{\sum_{i=1}^n y_i}\right)$$

(b) (5 points) Find the Fisher information  $\mathcal{I}(p)$ .

We start here by making the following assumptions:

- $p$  is an interior parameter value on the interval  $0 < p < 1$  such that derivatives exist and are finite.
- Support,  $y$ , is parameter independent and does not depend on  $p$ .
- Parameter is smooth such that for each  $y$ ,  $\ell$  is twice differentiable.
- We can exchange expectation and differentiation in this case.

Now, we can use the following definition for Fisher information:

$$\mathcal{I}(p) = -E[\ell''(p)].$$

So

$$\mathcal{I}(p) = -E\left[-\frac{n}{p^2} - \frac{\sum_{i=1}^n y_i - 1}{(1-p)^2}\right] = \frac{n}{p^2} + \frac{E[\sum_{i=1}^n y_i - 1]}{(1-p)^2}.$$

Since  $Y_i$  are i.i.d,

$$E\left[\sum_{i=1}^n y_i - 1\right] = nE[y - 1] = n\left(\frac{1}{p} - 1\right) = \frac{n(1-p)}{p}.$$

Substituting back in

$$\mathcal{I}(p) = \frac{n}{p^2} + \frac{n(1-p)}{p(1-p)^2} = \frac{n}{p^2} + \frac{n}{p(1-p)} = \frac{n}{p^2(1-p)}$$

(c) (5 points) Find the asymptotic variance (meaning, the approximate variance when the sample size  $n$  is large) of the maximum likelihood estimate.

Under regularity conditions, we know that

$$\sqrt{n}(\hat{p}_n - p) \xrightarrow{d} N\left(0, \frac{1}{I_1(p)}\right),$$

where  $I_1(p)$  is the Fisher information in one observation. Equivalently, since  $I_n(p) = nI_1(p)$ ,

$$\hat{p} \approx N\left(p, \frac{1}{I_n(p)}\right) \text{ for large } n.$$

From this it follows that:

$$\text{Var}(\hat{p}_n) \rightarrow \frac{1}{I_n(p)} \text{ as } n \rightarrow \infty.$$

At this point, we can plug in the Fisher information to obtain the asymptotic variance:

$$\text{Var}(\hat{p}_n) \approx \frac{1}{I_n(p)} = \frac{p^2(1-p)}{n}.$$

3. Consider an i.i.d. sample of size  $n$  from a  $N(\mu, \sigma^2)$  distribution.

- (a) (5 points) Show that the sample mean and sample variance make up a two-dimensional sufficient statistic for  $(\mu, \sigma^2)$ .

Let  $X_1, \dots, X_n \stackrel{\text{iid}}{\sim} N(\mu, \sigma^2)$ . The joint density of  $x = (x_1, \dots, x_n)$  is

$$f_{\mu, \sigma^2}(x_1, \dots, x_n) = \prod_{i=1}^n \frac{1}{\sqrt{2\pi\sigma^2}} \exp\left(-\frac{(x_i - \mu)^2}{2\sigma^2}\right) = (2\pi\sigma^2)^{-n/2} \exp\left(-\frac{1}{2\sigma^2} \sum_{i=1}^n (x_i - \mu)^2\right).$$

Using the identity

$$\sum_{i=1}^n (x_i - \mu)^2 = \sum_{i=1}^n (x_i - \bar{x})^2 + n(\bar{x} - \mu)^2,$$

and noting that

$$\sum_{i=1}^n (x_i - \bar{x})^2 = (n-1)s^2, \quad \text{where} \quad s^2 = \frac{1}{n-1} \sum_{i=1}^n (x_i - \bar{x})^2,$$

we obtain

$$f_{\mu, \sigma^2}(x_1, \dots, x_n) = (2\pi\sigma^2)^{-n/2} \exp\left(-\frac{(n-1)s^2 + n(\bar{x} - \mu)^2}{2\sigma^2}\right).$$

This can be written in the factorized form

$$f_{\mu, \sigma^2}(x_1, \dots, x_n) = \underbrace{(2\pi\sigma^2)^{-n/2} \exp\left(-\frac{(n-1)s^2}{2\sigma^2}\right)}_{g_{\mu, \sigma^2}(\bar{x}, s^2)} \exp\left(-\frac{n(\bar{x} - \mu)^2}{2\sigma^2}\right) \cdot \underbrace{1}_{h(x_1, \dots, x_n)}.$$

By the Neyman–Fisher factorization theorem, the statistic

$$T(X) = (\bar{X}, S^2)$$

is sufficient for  $(\mu, \sigma^2)$ .

- (b) (5 points) Suppose we know that  $\sigma^2 = 4$  but  $\mu$  unknown. Find a sufficient statistic for  $\mu$ .

The joint density of  $x = (x_1, \dots, x_n)$  is

$$f_{\mu}(x_1, \dots, x_n) = \prod_{i=1}^n \frac{1}{\sqrt{2\pi \cdot 4}} \exp\left(-\frac{(x_i - \mu)^2}{2 \cdot 4}\right) = (2\pi \cdot 4)^{-n/2} \exp\left(-\frac{1}{8} \sum_{i=1}^n (x_i - \mu)^2\right).$$

Again using the identity

$$\sum_{i=1}^n (x_i - \mu)^2 = \sum_{i=1}^n (x_i - \bar{x})^2 + n(\bar{x} - \mu)^2,$$

we obtain

$$f_{\mu}(x_1, \dots, x_n) = (2\pi \cdot 4)^{-n/2} \exp\left(-\frac{n(\bar{x} - \mu)^2}{8}\right) \exp\left(-\frac{1}{8} \sum_{i=1}^n (x_i - \bar{x})^2\right).$$

Hence

$$f_{\mu}(x_1, \dots, x_n) = \underbrace{(2\pi \cdot 4)^{-n/2} \exp\left(-\frac{n(\bar{x} - \mu)^2}{8}\right)}_{g_{\mu}(\bar{x})} \cdot \underbrace{\exp\left(-\frac{1}{8} \sum_{i=1}^n (x_i - \bar{x})^2\right)}_{h(x_1, \dots, x_n)}.$$

By the Neyman–Fisher factorization theorem,  $T(X) = \bar{X}$  is sufficient for  $\mu$ .

- (c) (5 points) Suppose we know that  $\mu = -3$  but  $\sigma^2$  is unknown. Find a sufficient statistic for  $\sigma^2$ .

The joint density of  $x = (x_1, \dots, x_n)$  is

$$f_{\sigma^2}(x_1, \dots, x_n) = \prod_{i=1}^n \frac{1}{\sqrt{2\pi\sigma^2}} \exp\left(-\frac{(x_i + 3)^2}{2\sigma^2}\right) = (2\pi\sigma^2)^{-n/2} \exp\left(-\frac{1}{2\sigma^2} \sum_{i=1}^n (x_i + 3)^2\right).$$

Let

$$T(X) = \sum_{i=1}^n (X_i + 3)^2.$$

Then

$$f_{\sigma^2}(x_1, \dots, x_n) = \underbrace{(2\pi\sigma^2)^{-n/2} \exp\left(-\frac{1}{2\sigma^2} T(x)\right)}_{g_{\sigma^2}(T(x))} \cdot \underbrace{1}_{h(x_1, \dots, x_n)}.$$

By the Neyman–Fisher factorization theorem,  $T(X) = \sum_{i=1}^n (X_i + 3)^2$  is sufficient for  $\sigma^2$ .

4. (10 points) A social scientist wanted to estimate the proportion of school children in Boston who live in a single-parent family. She decided to use a sample size such that, with probability 0.95, the error would not exceed 0.05. How large a sample size should she use, if she has no idea of the size of that proportion?

We want  $P(|\hat{p} - p| \leq 0.05) = 0.95$ . For a proportion, the margin of error is

$$E = z_{0.975} \sqrt{\frac{p(1-p)}{n}},$$

with  $z_{0.975} = 1.96$  for 95% confidence. Thus we need

$$1.96 \sqrt{\frac{p(1-p)}{n}} \leq 0.05.$$

Since  $p$  is unknown, we use the worst-case value  $p(1 - p) \leq 0.25$  (attained at  $p = 0.5$ ). Therefore,

$$1.96\sqrt{\frac{0.25}{n}} \leq 0.05.$$

Solving for  $n$ :

$$\sqrt{\frac{0.25}{n}} \leq \frac{0.05}{1.96}, \quad \frac{0.25}{n} \leq \left(\frac{0.05}{1.96}\right)^2,$$

$$n \geq \frac{0.25}{(0.05/1.96)^2} = 0.25 \left(\frac{1.96}{0.05}\right)^2 = 384.16.$$

Rounding up,

$$n = 385.$$

5. Consider collecting a sample of size  $n = 1497$  from a population with the goal of estimating the proportion of the population that prefers coffee rather than tea. Suppose that the true proportion is  $p = 0.53$ .

```
### Code shared between part (a) and part (b)

set.seed(123)

n <- 1497
p_true <- 0.53
s_vals <- c(5, 10, 100, 1000)

# function to estimate coverage for given confidence level
# and number of simulations
coverage_score_ci <- function(s, conf_level, n, p_true) {
  alpha <- 1 - conf_level
  z <- qnorm(1 - alpha/2)

  contain <- logical(s)

  for (i in 1:s) {

    x <- rbinom(1, size = n, prob = p_true)
    phat <- x / n

    se <- sqrt(phat * (1 - phat) / n)
    lower <- phat - z * se
    upper <- phat + z * se

    contain[i] <- (lower <= p_true && p_true <= upper)
```

```

}

mean(contain) * 100 # percent coverage
}

```

- (a) (10 points) Use R to simulate  $s$  different samples of size  $n$  from the population (using the true value of  $p$  to simulate the data). For each sample, construct a 95% score confidence interval for  $p$ . Report the percentage of the  $s$  confidence intervals that contain the true value of  $p$ . Do this for  $s = 5, 10, 100, 1000$ .

```

### 95% score (Wald) intervals
cat("95% score CI coverage (%)\\n")
for (s in s_vals) {
  cov <- coverage_score_ci(s, conf_level = 0.95, n
    = n, p_true = p_true)
  cat("s =", s, ":", round(cov, 1), "%\\n")
}

### 95% score CI coverage (%)
# s = 5 : 80 %
# s = 10 : 80 %
# s = 100 : 96 %
# s = 1000 : 95.4 %

```

- (b) (10 points) Repeat part [(a)], but this time construct 70% score confidence intervals.

```

### 70% score (Wald) intervals
cat("70% score CI coverage (%)\\n")
for (s in s_vals) {
  cov <- coverage_score_ci(s, conf_level = 0.70, n
    = n, p_true = p_true)
  cat("s =", s, ":", round(cov, 1), "%\\n")
}

### 70% score CI coverage (%)
# s = 5 : 80 %
# s = 10 : 90 %
# s = 100 : 70 %
# s = 1000 : 71.2 %

```

6. Consider a sample  $\mathbf{Y} = (Y_1, \dots, Y_n)$  that we wish to use to estimate the parameter  $\theta$ . Suppose that  $\theta_1(\mathbf{Y})$  is an estimator of  $\theta$  with  $E[(\theta_1(\mathbf{Y}))^2] < \infty$  for all  $\theta$ , suppose that  $T(\mathbf{Y})$  is a sufficient statistic for  $\theta$ , and let  $\theta_2(\mathbf{Y}) = E[\theta_1(\mathbf{Y})|T(\mathbf{Y})]$ . Then, for all  $\theta$ ,

$$E[(\theta_2(\mathbf{Y}) - \theta)^2] \leq E[(\theta_1(\mathbf{Y}) - \theta)^2],$$



and the inequality is strict unless  $\theta_1(\mathbf{Y}) = \theta_2(\mathbf{Y})$ .

- (a) (5 points) Note that  $\theta_1(\mathbf{Y})$  and  $\theta_2(\mathbf{Y})$  are both estimators of  $\theta$ . Interpret the statement above in the context of comparing the two estimators and what it implies about using sufficient statistics to construct estimators.

The construction

$$\theta_2(\mathbf{Y}) = \mathbb{E}[\theta_1(\mathbf{Y}) \mid T(\mathbf{Y})]$$

takes an arbitrary estimator  $\theta_1(\mathbf{Y})$  and *Rao-Blackwellizes* it by averaging out all sample-to-sample variation that is *irrelevant* once we know the sufficient statistic  $T(\mathbf{Y})$ . The displayed inequality

$$\mathbb{E}[(\theta_2(\mathbf{Y}) - \theta)^2] \leq \mathbb{E}[(\theta_1(\mathbf{Y}) - \theta)^2] \quad \text{for all } \theta$$

says that  $\theta_2$  has *no larger mean squared error* (MSE) than  $\theta_1$ , uniformly over the parameter space. In other words, conditioning on a sufficient statistic cannot make an estimator worse in MSE, and typically makes it strictly better. Practically, this implies:

- Sufficiency means  $T(\mathbf{Y})$  retains all information about  $\theta$  in the sample.
- Therefore, any dependence of  $\theta_1(\mathbf{Y})$  on  $\mathbf{Y}$  beyond what is captured by  $T(\mathbf{Y})$  is “noise” with respect to estimating  $\theta$ .
- Replacing  $\theta_1$  by  $\theta_2 = \mathbb{E}[\theta_1 \mid T]$  removes that extra noise, yielding an estimator at least as accurate (in MSE), with strict improvement unless  $\theta_1$  was already a function of  $T$  a.s.

- (b) **This question is only required for students enrolled in STAT 6530.** (10 points) Provide a proof of the statement above. Hints: First, show that the two estimators have the same means, so it suffices to compare their variances. To compare the variances of the estimators, recall the following result: if  $X$  and  $Z$  are random variables and  $X$  has finite variance, then  $\text{Var}(X) = E[\text{Var}(X|Z)] + \text{Var}(E[X|Z])$ .

Let  $\theta$  be fixed. Let  $T = T(\mathbf{Y})$  and define

$$\theta_2(\mathbf{Y}) = \mathbb{E}[\theta_1(\mathbf{Y}) \mid T].$$

First note that  $\theta_1$  and  $\theta_2$  have the same mean:

$$\mathbb{E}[\theta_2(\mathbf{Y})] = \mathbb{E}[\mathbb{E}[\theta_1(\mathbf{Y}) \mid T]] = \mathbb{E}[\theta_1(\mathbf{Y})],$$

by the tower property. Now compare the MSEs. Use the conditional-variance decomposition (law of total variance):

$$\text{Var}(\theta_1(\mathbf{Y})) = \mathbb{E}[\text{Var}(\theta_1(\mathbf{Y}) \mid T)] + \text{Var}(\mathbb{E}[\theta_1(\mathbf{Y}) \mid T]).$$

But  $\mathbb{E}[\theta_1(\mathbf{Y}) \mid T] = \theta_2(\mathbf{Y})$ , so

$$\text{Var}(\theta_1(\mathbf{Y})) = \mathbb{E}[\text{Var}(\theta_1(\mathbf{Y}) \mid T)] + \text{Var}(\theta_2(\mathbf{Y})) \geq \text{Var}(\theta_2(\mathbf{Y})).$$

Thus  $\text{Var}(\theta_2) \leq \text{Var}(\theta_1)$ . Next show that the two estimators have the same bias (hence the same squared bias). Since their expectations coincide,

$$\text{Bias}(\theta_2) = \mathbb{E}[\theta_2(\mathbf{Y})] - \theta = \mathbb{E}[\theta_1(\mathbf{Y})] - \theta = \text{Bias}(\theta_1).$$

Therefore,

$$\text{MSE}(\theta_i) = \mathbb{E}[(\theta_i(\mathbf{Y}) - \theta)^2] = \text{Var}(\theta_i(\mathbf{Y})) + \text{Bias}(\theta_i)^2, \quad i = 1, 2,$$

and since the biases are equal while  $\text{Var}(\theta_2) \leq \text{Var}(\theta_1)$ , we conclude

$$\mathbb{E}[(\theta_2(\mathbf{Y}) - \theta)^2] \leq \mathbb{E}[(\theta_1(\mathbf{Y}) - \theta)^2].$$

Finally, determine when the inequality is strict. From

$$\text{Var}(\theta_1(\mathbf{Y})) - \text{Var}(\theta_2(\mathbf{Y})) = \mathbb{E}[\text{Var}(\theta_1(\mathbf{Y}) \mid T)],$$

we have equality if and only if

$$\mathbb{E}[\text{Var}(\theta_1(\mathbf{Y}) \mid T)] = 0 \iff \text{Var}(\theta_1(\mathbf{Y}) \mid T) = 0 \text{ a.s.}$$

But  $\text{Var}(\theta_1 \mid T) = 0$  a.s. holds if and only if  $\theta_1(\mathbf{Y})$  is (a.s.) a function of  $T$ , equivalently

$$\theta_1(\mathbf{Y}) = \mathbb{E}[\theta_1(\mathbf{Y}) \mid T] = \theta_2(\mathbf{Y}) \quad \text{a.s.}$$

Hence the inequality is strict unless  $\theta_1(\mathbf{Y}) = \theta_2(\mathbf{Y})$  almost surely.  $\square$